

SC-646

Distributed Optimization and Machine Learning

Homework - 1

Name: Medhansh Sharma

Roll no.: 22b1287

February 2026

1 Primer on Strong Convexity

Proof. Let

$$\phi_x(z) = f(z) - \nabla f(x)^\top z \quad (1)$$

Take any $z_1, z_2 \in \mathbb{R}^d$ and $\lambda \in (0, 1)$. Then

$$\phi_x(\lambda z_1 + (1 - \lambda)z_2) = f(\lambda z_1 + (1 - \lambda)z_2) - \nabla f(x)^\top (\lambda z_1 + (1 - \lambda)z_2) \quad (2)$$

Since f is μ -strongly convex,

$$f(\lambda z_1 + (1 - \lambda)z_2) \leq \lambda f(z_1) + (1 - \lambda)f(z_2) - \frac{\mu}{2}\lambda(1 - \lambda)\|z_1 - z_2\|^2 \quad (3)$$

Substituting (3) into (2) and rearranging gives

$$\phi_x(\lambda z_1 + (1 - \lambda)z_2) \leq \lambda \phi_x(z_1) + (1 - \lambda)\phi_x(z_2) - \frac{\mu}{2}\lambda(1 - \lambda)\|z_1 - z_2\|^2 \quad (4)$$

Hence, ϕ_x is μ -strongly convex. A μ -strongly convex function satisfies the Polyak–Łojasiewicz inequality:

$$\frac{1}{2}\|\nabla \phi_x(y)\|^2 \geq \mu(\phi_x(y) - \phi_x^*) \quad (5)$$

where $\phi_x^* = \min_z \phi_x(z)$.

We compute

$$\nabla \phi_x(y) = \nabla f(y) - \nabla f(x) \quad (6)$$

At the minimizer y^* of ϕ_x , we have $\nabla \phi_x(y^*) = 0$, so

$$\nabla f(y^*) = \nabla f(x) \quad (7)$$

Since f is strongly convex, its gradient is injective, implying

$$y^* = x \quad (8)$$

Therefore,

$$\phi_x^* = \phi_x(x) = f(x) - \nabla f(x)^\top x \quad (9)$$

Substituting (6) and (9) into (5) yields

$$\frac{1}{2}\|\nabla f(y) - \nabla f(x)\|^2 \geq \mu(f(y) - \nabla f(x)^\top y - f(x) + \nabla f(x)^\top x) \quad (10)$$

Rearranging gives

$$f(y) \leq f(x) + \nabla f(x)^\top (y - x) + \frac{1}{2\mu}\|\nabla f(y) - \nabla f(x)\|^2 \quad (11)$$

This completes the proof.

2 AGD vs HB

Proof. We are given

$$f(x) = \log(x + \sqrt{1+x^2}) + x^2 \quad (1)$$

Computing the first derivative,

$$\nabla f(x) = \frac{1}{\sqrt{1+x^2}} + 2x \quad (2)$$

The second derivative is

$$\nabla^2 f(x) = -\frac{x}{(1+x^2)^{3/2}} + 2 \quad (3)$$

Let

$$g(x) = \frac{x}{(1+x^2)^{3/2}} \quad (4)$$

Then

$$\nabla^2 f(x) = 2 - g(x) \quad (5)$$

Differentiating $g(x)$,

$$g'(x) = \frac{1-2x^2}{(1+x^2)^{5/2}} \quad (6)$$

Setting $g'(x) = 0$, we obtain the critical points

$$x = \pm \frac{1}{\sqrt{2}} \quad (7)$$

Evaluating $g(x)$ at these points,

$$\max g(x) = \frac{2}{3\sqrt{3}}, \quad \min g(x) = -\frac{2}{3\sqrt{3}} \quad (8)$$

Hence,

$$\min \nabla^2 f(x) = 2 - \frac{2}{3\sqrt{3}} \quad (9)$$

Therefore f is μ -strongly convex with

$$\mu = 2 - \frac{2}{3\sqrt{3}} \approx 1.615 \quad (10)$$

For Lipschitz continuity of the gradient, we require

$$|\nabla^2 f(x)| \leq L \quad (11)$$

Using (10),

$$\max \nabla^2 f(x) = 2 + \frac{2}{3\sqrt{3}} \quad (12)$$

Thus ∇f is L -Lipschitz with

$$L = 2 + \frac{2}{3\sqrt{3}} \quad (13)$$

Hence, the function is strongly convex and admits a Lipschitz continuous gradient. Here's the link to the jupyter notebook implementing Accelerated Gradient Descent and Heavy-Ball Method: [Code for AGD and HB](#)

3 Contraction Coefficient

Proof. Consider gradient descent

$$x^{k+1} = G_\alpha(x^k) = x^k - \alpha \nabla f(x^k) \quad (1)$$

Let x^* denote the minimizer of f , so that

$$G_\alpha(x^*) = x^* \quad (2)$$

(a) Linear convergence under contraction

Assume G_α is a contraction:

$$\|G_\alpha(x) - G_\alpha(y)\| \leq L_G \|x - y\|, \quad L_G < 1 \quad (3)$$

Setting $y = x^*$ and using (2),

$$\|x^{k+1} - x^*\| = \|G_\alpha(x^k) - G_\alpha(x^*)\| \leq L_G \|x^k - x^*\| \quad (4)$$

By recursion,

$$\|x^k - x^*\| \leq L_G^k \|x^0 - x^*\| \quad (5)$$

Hence gradient descent converges linearly to x^* .

(b) Bound on the contraction coefficient

We write

$$G_\alpha(x) - G_\alpha(y) = (x - y) - \alpha(\nabla f(x) - \nabla f(y)) \quad (6)$$

By the Mean Value Theorem,

$$\nabla f(x) - \nabla f(y) = H(\xi)(x - y) \quad (7)$$

for some ξ on the line segment between x and y , where $\mu I \preceq H(\xi) \preceq LI$.

Substituting (7) into (6),

$$G_\alpha(x) - G_\alpha(y) = (I - \alpha H(\xi))(x - y) \quad (8)$$

Taking norms,

$$\|G_\alpha(x) - G_\alpha(y)\| \leq \|I - \alpha H(\xi)\| \|x - y\| \quad (9)$$

Since the eigenvalues of $H(\xi)$ lie in $[\mu, L]$,

$$\|I - \alpha H(\xi)\| \leq \max\{|1 - \alpha\mu|, |1 - \alpha L|\} \quad (10)$$

Thus the contraction coefficient satisfies

$$L_G \leq \max\{|1 - \alpha\mu|, |1 - \alpha L|\} \quad (11)$$

(c) Optimal step size

We minimize

$$\rho(\alpha) = \max\{|1 - \alpha\mu|, |1 - \alpha L|\} \quad (12)$$

The minimum occurs when the two terms are equal:

$$1 - \alpha\mu = \alpha L - 1 \quad (13)$$

Solving,

$$\alpha^* = \frac{2}{L + \mu} \quad (14)$$

Substituting into (12),

$$\rho^* = \frac{L - \mu}{L + \mu} \quad (15)$$

Let $\kappa = L/\mu$ be the condition number. Then

$$\rho^* = \frac{\kappa - 1}{\kappa + 1} \quad (16)$$

Using linear convergence from part (a),

$$\|x^{k+1} - x^*\| \leq \left(\frac{\kappa - 1}{\kappa + 1}\right)^{k+1} \|x^0 - x^*\| \quad (17)$$

4 Kernel SVMs

Here's the link to the jupyter notebook containing the code: [Code for Kernel SVMs](#)

5 Linear Convergence

Proof. Consider the proximal gradient update

$$x^{k+1} = \arg \min_y \left\{ \langle \nabla f(x^k), y - x^k \rangle + \frac{L}{2} \|y - x^k\|^2 + g(y) \right\} \quad (1)$$

From the L -smoothness of f , we have

$$f(x^{k+1}) \leq f(x^k) + \langle \nabla f(x^k), x^{k+1} - x^k \rangle + \frac{L}{2} \|x^{k+1} - x^k\|^2 \quad (2)$$

Adding $g(x^{k+1})$ to both sides gives

$$F(x^{k+1}) \leq F(x^k) + \langle \nabla f(x^k), x^{k+1} - x^k \rangle + \frac{L}{2} \|x^{k+1} - x^k\|^2 + g(x^{k+1}) - g(x^k) \quad (3)$$

By the definition of $D_g(x^k, L)$,

$$F(x^{k+1}) \leq F(x^k) - \frac{1}{2L} D_g(x^k, L) \quad (4)$$

Using the proximal-PL inequality,

$$D_g(x^k, L) \geq 2\mu(F(x^k) - F^*) \quad (5)$$

Substituting (5) into (4) yields

$$F(x^{k+1}) - F^* \leq F(x^k) - F^* - \frac{\mu}{L} (F(x^k) - F^*) \quad (6)$$

Therefore,

$$F(x^{k+1}) - F^* \leq \left(1 - \frac{\mu}{L}\right) (F(x^k) - F^*) \quad (7)$$

Hence F converges linearly with contraction coefficient

$$\rho = 1 - \frac{\mu}{L} \quad (8)$$

6 Necessity and Sufficiency of KKT Conditions

Proof. Consider the convex optimization problem

$$\min_x f(x) \quad \text{subject to} \quad g_i(x) \leq 0, \quad h_j(x) = 0$$

The Lagrangian is

$$\mathcal{L}(x, \lambda, \nu) = f(x) + \sum_i \lambda_i g_i(x) + \sum_j \nu_j h_j(x) \quad (1)$$

with $\lambda_i \geq 0$

Necessity

Suppose x^* and (λ^*, ν^*) are primal and dual optimal and strong duality holds. Then

$$f(x^*) = \inf_x \mathcal{L}(x, \lambda^*, \nu^*) \quad (2)$$

Hence x^* minimizes the Lagrangian, implying stationarity:

$$\nabla_x \mathcal{L}(x^*, \lambda^*, \nu^*) = 0 \quad (3)$$

Primal feasibility gives

$$g_i(x^*) \leq 0 \quad h_j(x^*) = 0 \quad (4)$$

Dual feasibility gives

$$\lambda_i^* \geq 0 \quad (5)$$

Complementary slackness follows from

$$\lambda_i^* g_i(x^*) = 0 \quad (6)$$

Thus the KKT conditions hold.

Sufficiency

Suppose x^* and (λ^*, ν^*) satisfy KKT conditions. By convexity of f and g_i and linearity of h_j ,

$$f(x) \geq f(x^*) + \sum_i \lambda_i^* g_i(x) + \sum_j \nu_j^* h_j(x) = \mathcal{L}(x, \lambda^*, \nu^*) \quad (7)$$

Taking infimum over x gives

$$p^* \geq d^*. \quad (8)$$

Since weak duality always gives $d^* \leq p^*$ and strong duality holds, we conclude

$$p^* = d^* = f(x^*) \quad (9)$$

Hence x^* and (λ^*, ν^*) are optimal.

Therefore, KKT conditions are necessary and sufficient for optimality.

7 KKT conditions in action

Solution. Consider the optimization problem

$$\max_{x, y \geq 0} xy \quad \text{subject to} \quad x + y^2 \leq 2$$

We convert it to a minimization problem:

$$\begin{aligned} \min_{x, y \geq 0} -xy \quad \text{subject to} \quad & g_1(x, y) = x + y^2 - 2 \leq 0, \\ & g_2(x, y) = -x \leq 0, \quad g_3(x, y) = -y \leq 0 \end{aligned}$$

The Lagrangian is

$$\mathcal{L}(x, y, \lambda) = -xy + \lambda_1(x + y^2 - 2) - \lambda_2 x - \lambda_3 y \quad (1)$$

where $\lambda_i \geq 0$.

KKT stationarity conditions

$$\frac{\partial \mathcal{L}}{\partial x} = -y + \lambda_1 - \lambda_2 = 0 \quad (2)$$

$$\frac{\partial \mathcal{L}}{\partial y} = -x + 2\lambda_1 y - \lambda_3 = 0 \quad (3)$$

Complementary slackness

$$\lambda_1(x + y^2 - 2) = 0, \quad \lambda_2 x = 0, \quad \lambda_3 y = 0 \quad (4)$$

Since we are maximizing xy , the optimal solution must satisfy $x > 0$ and $y > 0$. Hence from complementary slackness,

$$\lambda_2 = \lambda_3 = 0 \quad (5)$$

From (2), we obtain

$$\lambda_1 = y \quad (6)$$

Substituting into (3) gives

$$-x + 2y^2 = 0 \quad \Rightarrow \quad x = 2y^2 \quad (7)$$

Because $\lambda_1 > 0$, the first constraint is active:

$$x + y^2 = 2 \quad (8)$$

Substituting $x = 2y^2$ into (8),

$$2y^2 + y^2 = 2 \quad \Rightarrow \quad 3y^2 = 2 \quad \Rightarrow \quad y = \sqrt{\frac{2}{3}} \quad (9)$$

Hence

$$x = 2y^2 = \frac{4}{3} \quad (10)$$

The optimal value is

$$f^* = xy = \frac{4}{3} \sqrt{\frac{2}{3}} \quad (11)$$

Therefore, the optimal solution is

$$(x^*, y^*) = \left(\frac{4}{3}, \sqrt{\frac{2}{3}} \right)$$

8 Condition for Convexity

Proof. We are given for all $x, y \in \mathbb{R}^d$,

$$f(y) \geq f(x) + \nabla f(x)^\top (y - x) \quad (1)$$

Let $\lambda \in (0, 1)$ and define

$$z = \lambda x + (1 - \lambda)y \quad (2)$$

Applying (1) with (x, z) replaced by (z, y) gives

$$f(y) \geq f(z) + \nabla f(z)^\top (y - z) \quad (3)$$

Similarly, applying (1) with (x, z) replaced by (z, x) yields

$$f(x) \geq f(z) + \nabla f(z)^\top (x - z) \quad (4)$$

Multiplying (3) by $(1 - \lambda)$ and (4) by λ , we obtain

$$(1 - \lambda)f(y) \geq (1 - \lambda)f(z) + (1 - \lambda)\nabla f(z)^\top (y - z) \quad (5)$$

$$\lambda f(x) \geq \lambda f(z) + \lambda \nabla f(z)^\top (x - z) \quad (6)$$

Adding (5) and (6) gives

$$\lambda f(x) + (1 - \lambda)f(y) \geq f(z) + \nabla f(z)^\top (\lambda(x - z) + (1 - \lambda)(y - z)) \quad (7)$$

Using the definition of z in (2), we have

$$\lambda(x - z) + (1 - \lambda)(y - z) = 0 \quad (8)$$

Substituting (8) into (7) yields

$$\lambda f(x) + (1 - \lambda)f(y) \geq f(z) \quad (9)$$

Finally, using (2) again,

$$f(\lambda x + (1 - \lambda)y) \leq \lambda f(x) + (1 - \lambda)f(y) \quad (10)$$

Therefore, f is convex.